Core/Eval/Soundness.lean
@@ -67,21 +67,30 @@ theorem pattern_match_sound {m : Nat} {cs : Vec Constructor m} {ps : Pattern m'}
 intro h
 fun_induction pattern_match <;> simp at *
 apply Pattern.Match.nil
-case _ ih =>
+· case _ ih =>
   unfold pattern_match at h
   simp at h; rcases h with ⟨⟨⟨⟨h1, h2⟩, h3⟩, h4⟩, h5⟩
   subst h5; subst h4; subst h3; subst h2;
   replace ih := ih h1
-  push_cast; norm_cast
   sorry
 
-sorry
+· sorry
+
+theorem get_match_sound {ctors : Vec Constructor m} {ps : Vec (Pattern m) n}:
+  get_match ctors ps = some i ->
+  Pattern.Match ctors (ps[i])
+ := by
+ intro h
+ unfold get_match at h
+ replace h := Vec.findIdx_sound h
+ replace h := pattern_match_sound h
+ simp at h; apply h
 
 theorem eval_sound (Γ : GlobalEnv) :
   M.eval Γ = some N ->
   Γ ⊢ M ~> N := by
 intro h
-fun_induction Term.eval <;> simp at h
+fun_induction Term.eval generalizing N <;> simp at h
 case _ =>  -- lookup defn
   rw[Option.bind_eq_some_iff] at h; rcases h with ⟨h1, h2, h⟩
   cases h;
@@ -101,53 +110,111 @@ case _ ih => -- openm
   · apply h5
   · simp; symm at h; apply h
 
-case _ => -- openm
-  sorry
+case _ ss _ i j ih1 ih2 => -- openm
+  rw[Option.bind_eq_some_iff] at h; rcases h with ⟨h1, h2, h⟩
+  simp at h; rcases h with ⟨h3, h4⟩
 
-case _ => -- mtch
-  sorry
+  replace j := Vec.findIdx_sound j
+  rw[Option.isSome_iff_exists] at j; rcases j with ⟨t', j⟩
+  rw[h3] at j; simp at j; subst h1
+  replace ih2 := ih2 h2
+  replace ih1 := ih1 i h2
+  subst N
+  apply Red.openm_congr i
+  · have e1 := Vec.to_get_elem (ss.to.set i t') i
+    have e2 := Vec.get_set_eq (x := t') (v := ss.to) (i := i)
+    rw[e1, e2]; apply ih1
+  · intro j h;
+    replace h : i ≠ j := by grind
+    have lem := Vec.get_set_neq h (x := t') (v := ss.to)
+    symm at lem
+    simp [<-Vec.to_get_elem] at lem; apply lem
 
-case _ => -- mtch
-  sorry
+
+case _ ih => -- mtch
+  rw[Option.bind_eq_some_iff] at h; rcases h with ⟨h1, h2, h⟩
+  rw[Option.bind_eq_some_iff] at h; rcases h with ⟨i, h4, h⟩
+  simp at h; symm at h
+  replace h2 := Term.is_data_sound h2
+  replace h4 := get_match_sound h4; rw[<-Fun.Vec.to_get_elem] at h4
+  apply Red.data_match (i := i)
+  · apply h2
+  · apply h4
+  · apply h
+
+case _ ss _ _ m_ss i j ih1 ih2 => -- mtch congr
+  rw[Option.bind_eq_some_iff] at h; rcases h with ⟨h1, h2, h⟩
+  simp at h; subst h
+  replace ih2 := ih2 h2
+  apply Red.match_congr
+  · have e1 := Vec.to_get_elem (ss.to.set i h1) i;
+    have e2 := Vec.get_set_eq (x := h1) (v := ss.to) (i := i)
+    rw[e1, e2]; apply ih2
+  · intro j h;
+    replace h : i ≠ j := by grind
+    have lem := Vec.get_set_neq h (x := h1) (v := ss.to)
+    symm at lem; simp [<-Vec.to_get_elem] at lem; apply lem
+
 
 case _ => -- Λ[K] t •[T]
-  sorry
+  subst N; constructor
 
-case _ => -- t •[T]
-  sorry
+case _ ih => -- t •[T]
+  rw[Option.bind_eq_some_iff] at h; rcases h with ⟨h1, h2, h⟩
+  simp at h; subst N
+  constructor; apply ih h2
 
-case _ => -- λ t • t
-  sorry
+case _ => -- prj 0 app
+  subst N; apply Red.prj_fst_app
 
-case _ => -- t • t
-  sorry
+case _ => -- prj0 ->
+  subst N; apply Red.prj_fst_arr
 
-case _ =>
-  sorry
+case _ => -- prj 1 app
+  subst h
+  apply Red.prj_snd_app
 
-case _ =>
-  sorry
+case _ => -- prj 1 arrow
+  subst h
+  apply Red.prj_snd_arr
 
-case _ =>
-  sorry
+case _ ih => -- prj congr
+  rw[Option.bind_eq_some_iff] at h; rcases h with ⟨t', h1, h⟩
+  simp at h; subst N
+  replace ih := ih h1
+  apply Red.ctor1_congr ih
 
-case _ =>
-  sorry
+case _ => -- β
+  subst N
+  apply Red.beta
 
-case _ =>
-  sorry
-case _ =>
-  sorry
+case _ ih1 => -- t1 • t2 ~> t1' • t2
+  rw[Option.bind_eq_some_iff] at h; rcases h with ⟨t', h2, h⟩
+  simp at h; subst N
+  replace ih1 := ih1 h2
+  apply Red.app_congr ih1
 
-case _ =>
-  sorry
-case _ =>
-  sorry
+case _ => -- ∀c[refl] •c[refl]
+  subst h; apply Red.apptc
 
-case _ =>
-  sorry
-case _ =>
-  sorry
+case _ ih =>
+  subst N
+  apply Red.apptc_congr2;
+  apply ih; assumption
 
+case _ ih =>
+  subst h;
+  apply Red.apptc_congr1
+  apply ih; assumption
+
+
+case _ => -- t ▸ refl A ~> t
+  subst h
+  constructor
+
+case _ ih =>
+  rw[Option.bind_eq_some_iff] at h; rcases h with ⟨h1, h2, h⟩
+  simp at h; subst N
+  apply Red.cast_congr; apply ih h2
 
 end Core
